Complete another admitted proof

LinearScan/Lib.hs
@@ -46,28 +46,26 @@ foldl_with_index f b v =
       (:) y ys -> go ((Prelude.succ) n) ys (f n z y)}}
   in go 0 v b
 
-dep_foldl_inv' :: (a1 -> Eqtype.Equality__Coq_type) -> a1 -> ([]
-                  Eqtype.Equality__Coq_sort) -> Prelude.Int -> (a1 -> []
-                  Eqtype.Equality__Coq_sort) -> (a1 -> a1 -> () ->
-                  Eqtype.Equality__Coq_sort -> Eqtype.Equality__Coq_sort) ->
-                  (a1 -> () -> Eqtype.Equality__Coq_sort -> ([]
-                  Eqtype.Equality__Coq_sort) -> () -> Specif.Coq_sig2 
-                  a1) -> a1
-dep_foldl_inv' e b v n q f f0 =
-  let {filtered_var = (,) (LinearScan.Utils.uncons v) n} in
+dep_foldl_inv :: (a1 -> Eqtype.Equality__Coq_type) -> a1 -> ([]
+                 Eqtype.Equality__Coq_sort) -> Prelude.Int -> (a1 -> []
+                 Eqtype.Equality__Coq_sort) -> (a1 -> a1 -> () ->
+                 Eqtype.Equality__Coq_sort -> Eqtype.Equality__Coq_sort) ->
+                 (a1 -> () -> Eqtype.Equality__Coq_sort -> ([]
+                 Eqtype.Equality__Coq_sort) -> () -> Specif.Coq_sig2 
+                 a1) -> a1
+dep_foldl_inv e b v n q f f0 =
+  let {filtered_var = (,) v n} in
   case filtered_var of {
-   (,) s n0 ->
-    case s of {
-     Prelude.Just s0 ->
-      case s0 of {
-       (,) y s1 ->
-        (\fO fS n -> if n Prelude.== 0 then fO () else fS (n Prelude.- 1))
-          (\_ ->
-          b)
-          (\n' ->
-          let {filtered_var0 = f0 b __ y s1 __} in
-          let {ys' = Prelude.map (f b filtered_var0 __) s1} in
-          dep_foldl_inv' e filtered_var0 ys' n' q f f0)
-          n0};
-     Prelude.Nothing -> b}}
+   (,) l n0 ->
+    case l of {
+     [] -> b;
+     (:) y ys ->
+      (\fO fS n -> if n Prelude.== 0 then fO () else fS (n Prelude.- 1))
+        (\_ ->
+        b)
+        (\n' ->
+        let {filtered_var0 = f0 b __ y ys __} in
+        let {ys' = Prelude.map (f b filtered_var0 __) ys} in
+        dep_foldl_inv e filtered_var0 ys' n' q f f0)
+        n0}}
 
